Core/Metatheory/GlobalWf.lean
@@ -9,59 +9,279 @@ import Core.Global
 
 namespace Core
 theorem GlobalWf.drop_wf : ∀ n, ⊢ G -> ⊢ G.drop n := by
-intro n wf
-induction wf generalizing n
-case _ => simp; constructor
-case _ g gwf wf ih =>
-induction n
-case _ => simp; constructor; assumption; assumption
-case _ => simp; apply ih
+  intro n wf
+  induction wf generalizing n
+  case _ => simp; constructor
+  case _ g gwf wf ih =>
+  induction n
+  case _ => simp; constructor; assumption; assumption
+  case _ => simp; apply ih
 
+theorem GlobalWf.drop_lookup_unique_vec :
+  (∀ i, v i = none) ->
+  Vec.fold Option.or (lookup x G) v = lookup x G
+:= by
+  intro h
+  induction v using Vec.induction
+  case _ => simp
+  case _ hd tl ih =>
+    simp; have lem := h 0; simp at lem
+    subst lem; simp
+    rw [ih]; intro i
+    apply h (Fin.succ i)
 
-theorem Global.drop_lookup {G : List Global} :
+theorem GlobalWf.drop_lookup_unique {G : List Global} n :
+  ⊢ G ->
+  lookup x (G.drop n) = some t ->
+  lookup x G = some t
+:= by
+  intro wf j
+  induction wf generalizing n <;> simp at *
+  case nil => exact j
+  case cons G j1 j2 wf ih =>
+    cases n <;> simp at *
+    case zero => exact j
+    case succ n =>
+      replace ih := ih n j
+      cases j2
+      case data n y K ctors ctors' j1 j2 j3 j4 =>
+        simp [lookup]; split
+        case _ e => subst e; rw [ih] at j4; injection j4
+        case _ e =>
+          rw [drop_lookup_unique_vec]; exact ih
+          intro i
+          generalize endef : ctors i = en at *
+          rcases en with ⟨z, A⟩; simp; intro e2; subst e2
+          replace j3 := j3 i x A endef
+          rcases j3 with ⟨j3, j4, j5⟩
+          simp [lookup] at j5; split at j5
+          case _ e2 => apply e e2
+          case _ e2 => rw [ih] at j5; injection j5
+      case openm T b y j1 j2 =>
+        simp [lookup]; split
+        case _ e => subst e; rw [ih] at j2; injection j2
+        case _ e => exact ih
+      case opent y j1 j2 =>
+        simp [lookup]; split
+        case _ e => subst e; rw [ih] at j2; injection j2
+        case _ e => exact ih
+      case defn T b t' y j1 j2 j3 =>
+        simp [lookup]; split
+        case _ e => subst e; rw [ih] at j3; injection j3
+        case _ e => exact ih
+      case inst y T t' j1 j2 => simp [lookup]; exact ih
+      case instty y T j1 j2 =>
+        simp [lookup]; split
+        case _ e => subst e; rw [ih] at j2; injection j2
+        case _ e => exact ih
+
+theorem GlobalWf.drop_lookup_impossible {G : List Global} :
   ⊢ G ->
   G' = G.drop n ->
-  lookup x G' = t ->
-  lookup x G = t' ->
-  t = t' := by
-intro wf e h1 h2
-induction n generalizing G G' t t' <;> simp at *
-case zero => subst e; rw[h1] at h2; assumption
-case succ n ih =>
-  cases G <;> simp at *
-  case nil =>
-    simp [lookup] at h1 h2
-    subst e h1 h2; simp [lookup]
-  case cons g G =>
-    apply @ih G' t t' G _ e h1 _
-    cases wf; case _ wf _ => exact wf
-    sorry
+  lookup x G' = some t ->
+  lookup x G = none ->
+  False
+:= by
+  intro wf e h1 h2
+  subst e; replace h1 := drop_lookup_unique n wf h1
+  rw [h2] at h1; injection h1
 
-
-
-theorem Kinding.arbitrary_weakening_global : ⊢ G ->
+theorem GlobalWf.drop_lookup {G : List Global} n :
+  ⊢ G ->
   G' = G.drop n ->
-  (G'& Δ ⊢ T : K) ->
-  G&Δ ⊢ T : K := by
-intro wf e j
-induction j generalizing G
-case var =>
-  apply Kinding.var; assumption
-case global x K Δ h =>
-  apply Kinding.global
-  simp [lookup_kind] at *;
-  generalize zdef : lookup  x G = z at *
-  generalize zdef' : lookup x G' = z' at *
-  have lem := Global.drop_lookup wf e zdef' zdef
-  subst z'; rw[lem] at h; assumption
-case all j ih =>
-  replace ih := @ih G wf e
-  apply Kinding.all; assumption
-all_goals (case _ ih1 ih2 =>
-  replace ih1 := @ih1 G wf e
-  replace ih2 := @ih2 G wf e
-  constructor; assumption; assumption)
+  lookup x G' = some t ->
+  lookup x G = some t' ->
+  t = t'
+:= by
+  intro wf e h1 h2
+  subst e; replace h1 := drop_lookup_unique n wf h1
+  have lem := Global.lookup_unique h1 h2
+  injection lem
 
+theorem Kinding.drop_weaken_global n :
+  ⊢ G ->
+  G' = G.drop n ->
+  G'& Δ ⊢ T : K ->
+  G&Δ ⊢ T : K
+:= by
+  intro wf e j
+  induction j generalizing G
+  case var =>
+    apply Kinding.var; assumption
+  case global x K Δ h =>
+    apply Kinding.global
+    simp [lookup_kind] at *;
+    generalize zdef  : lookup x G = z at *
+    generalize zdef' : lookup x G' = z' at *
+    cases z'; simp at h; case _ z' =>
+    cases z; simp at h
+    case none =>
+      exfalso
+      apply GlobalWf.drop_lookup_impossible wf e zdef' zdef
+    case some z =>
+      have lem := GlobalWf.drop_lookup n wf e zdef' zdef
+      subst z'; assumption
+  case all j ih =>
+    replace ih := @ih G wf e
+    apply Kinding.all; assumption
+  all_goals (case _ ih1 ih2 =>
+    replace ih1 := @ih1 G wf e
+    replace ih2 := @ih2 G wf e
+    constructor; assumption; assumption)
+
+theorem Typing.drop_weaken_global n :
+  ⊢ G ->
+  G' = G.drop n ->
+  G'&Δ,Γ ⊢ t : T ->
+  G&Δ,Γ ⊢ t : T
+:= by
+  intro wf e j
+  induction j generalizing G
+  case var => sorry
+  case global x A Δ b Γ j1 j2 =>
+    sorry
+    -- apply global; simp [lookup_type] at *
+    -- generalize zdef  : lookup x G = z at *
+    -- generalize zdef' : lookup x G' = z' at *
+    -- have lem := GlobalWf.drop_lookup n wf e zdef' zdef
+    -- subst z'; rw [lem] at j1; exact j1
+    -- apply Kinding.drop_weaken_global n wf e j2
+  case mtch => sorry
+  case guard => sorry
+  case lam => sorry
+  case app => sorry
+  case lamt => sorry
+  case appt => sorry
+  case cast => sorry
+  case refl => sorry
+  case sym => sorry
+  case seq => sorry
+  case appc => sorry
+  case arrowc => sorry
+  case fst => sorry
+  case snd => sorry
+  case allc => sorry
+  case apptc => sorry
+  case zero j =>
+    apply zero
+    apply Kinding.drop_weaken_global n wf e j
+  case choice => sorry
+
+theorem ValidInstTy.drop_weaken_global n :
+  ⊢ G ->
+  G' = G.drop n ->
+  ValidInstTy G' x Δ A ->
+  ValidInstTy G x Δ A
+:= by
+  intro wf e j
+  induction j generalizing G
+  case base j1 j2 =>
+    apply ValidInstTy.base j1
+    apply Kinding.drop_weaken_global n wf e j2
+  case all j1 j2 ih =>
+    apply ValidInstTy.all
+    apply Kinding.drop_weaken_global n wf e j1
+    apply ih wf e
+  case arrow j1 j2 ih =>
+    apply ValidInstTy.arrow
+    apply ih wf e
+    apply Kinding.drop_weaken_global n wf e j2
+
+theorem GlobalWf.lookup_weaken :
+  ⊢ (e1::G) ->
+  lookup x G = some e2 ->
+  lookup x (e1::G) = some e2
+:= by
+  intro wf j
+  apply drop_lookup_unique 1 wf
+  simp; exact j
+
+theorem EntryWf.weaken :
+  ⊢ (e1::G) ->
+  EntryWf G e2 ->
+  EntryWf (e1::G) e2
+:= by
+  intro wf j
+  induction j
+  case data j =>
+    apply EntryWf.data
+    apply GlobalWf.lookup_weaken wf j
+  case ctor j1 j2 j3 =>
+    apply EntryWf.ctor
+    apply Kinding.drop_weaken_global 1 wf (by simp) j1
+    apply j2
+    apply GlobalWf.lookup_weaken wf j3
+  case opent j1 j2 =>
+    apply EntryWf.opent j1
+    apply GlobalWf.lookup_weaken wf j2
+  case openm j1 j2 =>
+    apply EntryWf.openm
+    apply Kinding.drop_weaken_global 1 wf (by simp) j1
+    apply GlobalWf.lookup_weaken wf j2
+  case defn j1 j2 j3 j4 =>
+    apply EntryWf.defn
+    apply Kinding.drop_weaken_global 1 wf (by simp) j2
+    apply Typing.drop_weaken_global 1 wf (by simp) j3
+    apply GlobalWf.lookup_weaken wf j4
+  case instty j1 j2 =>
+    apply EntryWf.instty
+    apply ValidInstTy.drop_weaken_global 1 wf (by simp) j1
+    apply GlobalWf.lookup_weaken wf j2
+
+theorem EntryWf.from_lookup :
+  ⊢ G ->
+  lookup x G = some e ->
+  EntryWf G e
+:= by
+  intro wf h
+  induction wf generalizing e
+  case nil => simp [lookup] at h
+  case cons G g gwf wf ih =>
+    have gwf' := gwf
+    have wf' := ListGlobalWf.cons gwf' wf
+    cases gwf <;> simp [lookup] at h
+    case data j1 j2 j3 j4 =>
+      split at h
+      case _ e1 =>
+        subst e1; injection h with e; subst e
+        apply EntryWf.data; simp [lookup]
+      case _ e1 =>
+
+        sorry
+    case opent j1 j2 =>
+      split at h
+      case _ e1 =>
+        subst e1; injection h with e; subst e
+        apply EntryWf.opent j1; simp [lookup]
+      case _ e1 => apply weaken wf' (ih h)
+    case openm j1 j2 =>
+      split at h
+      case _ e1 =>
+        subst e1; injection h with e; subst e
+        apply EntryWf.openm
+        apply Kinding.drop_weaken_global 1 wf' (by simp) j1
+        simp [lookup]
+      case _ e1 => apply weaken wf' (ih h)
+    case defn j1 j2 j3 =>
+      split at h
+      case _ e1 =>
+        subst e1; injection h with e; subst e
+        apply EntryWf.defn
+        apply Kinding.drop_weaken_global 1 wf' (by simp) j1
+        apply Typing.drop_weaken_global 1 wf' (by simp) j2
+        simp [lookup]
+      case _ e1 => apply weaken wf' (ih h)
+    case inst j1 j2 =>
+
+      sorry
+    case instty j1 j2 =>
+      split at h
+      case _ e1 =>
+        subst e1; injection h with e; subst e
+        apply EntryWf.instty
+        apply ValidInstTy.drop_weaken_global 1 wf' (by simp) j1
+        simp [lookup]
+      case _ e1 => apply weaken wf' (ih h)
 
 theorem EntryWf.get_openm {G} {Δ} {Γ} :
    ⊢ G ->
@@ -79,107 +299,42 @@ constructor
   assumption; assumption
 · exists bk
 
--- theorem GlobalWf.weaken_defn :
---   ⊢ G ->
---   GlobalWf G (.defn x T t) ->
---   G&Δ, Γ ⊢ t : A ->
---   (.defn x T t :: G)&Δ, Γ ⊢ t : A := by
--- intro wf wfe j
--- induction j <;> (simp at *; cases wfe)
--- case var j => cases j <;> simp at *
--- case global j => sorry
--- case mtch => sorry
--- sorry
--- sorry
--- sorry
--- sorry
--- sorry
--- sorry
--- sorry
--- sorry
--- sorry
--- sorry
--- sorry
--- sorry
--- sorry
--- sorry
--- sorry
--- sorry
--- sorry
-
--- theorem GlobalWf.weaken_type :
---   ⊢ G ->
---   GlobalWf G e ->
---   Δ = [] ->
---   G&Δ ⊢ T : K ->
---   (e :: G)&Δ ⊢ T : K := by
--- intro wf wfe e j
--- cases wfe
--- case data =>
---   induction j
---   case var => subst e; simp at *
---   case global => sorry
---   case arrow => sorry
---   case all => sorry
---   case eq => sorry
---   case app => sorry
-
--- case opent K y _ h =>
---   induction j
---   case var => subst e; simp at *
---   case global x K' _ h1 =>
---     apply Kinding.global
---     unfold lookup_kind
---     generalize zdef : lookup x (.opent y K :: G) = z at *
---     cases z;
---     case _ =>
---       simp; simp [lookup] at zdef;
---       split at zdef
---       case _ e =>
---         subst e; simp [lookup_kind] at h1; rw[h] at h1; simp at h1
---       case _ =>  simp [lookup_kind] at h1; rw[zdef] at h1; simp at h1
---     case _ z =>
---       simp; unfold lookup at zdef
---       split at zdef
---       case _ e =>
---         replace e := eq_of_beq e; subst e; simp at zdef; simp[lookup_kind] at h1; rw[h] at h1; simp at h1
---       case _ => simp[lookup_kind] at h1; rw[zdef] at h1; simp at h1; assumption
---   case arrow j1 j2 ih1 ih2 =>
---     apply Kinding.arrow
---     apply ih1 e
---     apply ih2 e
---   case all ih1 =>
---     subst e
---     sorry -- booo!!
---   case eq => sorry
---   case app => sorry
-
--- case openm => sorry
--- case inst => sorry
--- case defn => sorry
--- case instty => sorry
-
-
-
-
 theorem GlobalWf.types_have_base_kind :
   ⊢ G ->
   lookup_type G x = some T ->
-  ∃ b, G&Δ ⊢ T : .base b := by
-intro wf h
--- generalize lkdef : lookup_type G x = lk at *
-induction wf generalizing x T
-case _ => simp [lookup_type, lookup, default] at *
-case _ G g gwf wf ih =>
-  replace ih := @ih x T
+  ∃ b, G&Δ ⊢ T : .base b
+:= by
+  intro wf h
+  -- generalize lkdef : lookup_type G x = lk at *
+  induction wf generalizing x T
+  case _ => simp [lookup_type, lookup, default] at *
+  case _ G g gwf wf ih =>
+    replace ih := @ih x T
+    have gwf' := gwf
+    cases gwf <;> simp [lookup_type, lookup] at h
+    case data => sorry
+    case opent K y h1 h2 =>
+      replace h := get!_option2_eq_some h
+      obtain ⟨w, q1, q2⟩ := Option.map_eq_some_iff.1 h
+      clear h; split at q1
+      case _ e =>
+        subst e; injection q1 with e; subst e
+        simp [Entry.type] at q2
+      case _ e =>
+        have lem := lookup_type_reconstruct q1 q2
+        obtain ⟨b, ih⟩ := ih lem
+        exists b; apply Kinding.arbitrary_weakening_global (n := 1) _ (by simp) ih
+        apply ListGlobalWf.cons gwf' wf
+    case openm => sorry
+    case defn => sorry
+    case inst => sorry
+    case instty =>
+      sorry
 
-  sorry
-
-
-theorem wf_lookup_type_sound :
+theorem GlobalWf.lookup_type_sound :
   ⊢ G ->
   lookup_type G x = some T ->
-  G&Δ, Γ ⊢ g#x : T := by
+  G&Δ,Γ ⊢ g#x : T := by
  intro wf h
  have lem := GlobalWf.types_have_base_kind (Δ := Δ) wf h;
  rcases lem with ⟨bk, lem⟩
@@ -189,11 +344,17 @@ theorem wf_lookup_type_sound :
 theorem GlobalWf.lookup_defn_type_exists {G : List Global} {Δ : List Kind} {Γ : List Ty} :
   ⊢ G ->
   lookup_defn G x = some t ->
-  ∃ T b, lookup_type G x = some T ∧ G&Δ ⊢ T : .base b := by
-intro wf h
-unfold lookup_defn at h
-generalize zdef : lookup x G = z at *
-sorry
+  ∃ T b, lookup_type G x = some T ∧ G&Δ ⊢ T : .base b
+:= by
+  intro wf h
+  unfold lookup_defn at h; simp at h
+  obtain ⟨w, q1, q2⟩ := Option.bind_eq_some_iff.1 h; clear h
+  cases w <;> simp at q2; case _ y A t' =>
+  subst q2
+  have lem : lookup_type G x = some A := by
+    simp [lookup_type]; rw [q1]; simp [Entry.type]
+  obtain ⟨b, h⟩ := types_have_base_kind (Δ := Δ) wf lem
+  exists A; exists b
 
 theorem GlobalWf.lookup_defn_type {G : List Global} {Δ : List Kind} {Γ : List Ty} :
   ⊢ G ->
@@ -204,7 +365,7 @@ have lem := GlobalWf.lookup_defn_type_exists (G := G) (Δ := Δ) (Γ := Γ) wf h
 rcases lem with ⟨T, b, lem1, lem2⟩
 exists T; exists b
 constructor
-· sorry
+· apply lookup_type_sound wf lem1
 · sorry
 
 end Core
